MyVector.v
@@ -1,0 +1,82 @@
+Require Export Vector.
+Require Import Eqdep.
+Import VectorNotations.
+
+Set Implicit Arguments.
+Unset Strict Implicit.
+
+Section Fin.
+  Lemma finvS (n : nat) (i : Fin.t (S n)) : (i = Fin.F1 \/ exists i', i = Fin.FS i').
+  Proof.
+    pattern n, i; apply (Fin.caseS).
+    - intros n0; tauto.
+    - intros n0 p; right; eexists; tauto.
+  Qed.
+
+Lemma fin_eq_dec : forall (n : nat) (i j : Fin.t n), {i = j} + {i <> j}.
+Proof.
+  refine (
+      fun n =>
+        match n with
+          | O => fun (i _ : Fin.t 0) => match (Fin.case0 (fun _ => False) i) with end
+          | S n => 
+            Fin.rect2 (fun n (i : Fin.t n) (j : Fin.t n) => {i = j} + {i <> j})
+                      (fun n => left _ _)
+                      (fun n f => right _ _)
+                      (fun n f =>  right _ _)
+                      (fun n f g (b : {f = g} + {f <> g}) => if b then left _ _ else right _ _)
+        end); subst; try inversion 1; eauto.
+  apply inj_pair2 in H1; congruence.
+Qed.
+End Fin.
+
+Section Vector.
+  Variable T : Type.
+  Variable n : nat.
+
+  Lemma vec_exvec (P : Fin.t n -> T -> Prop) : 
+    (forall i : Fin.t n, exists x : T, P i x) -> 
+    exists v : Vector.t T n, forall i : Fin.t n, P i v[@i].
+  Proof.
+    induction n as [|n']; [exists []; inversion 0 | intros H].
+    destruct n' as [|n'']; [destruct (H Fin.F1) as [x Hx]; exists [x] | ].
+    - intros i; destruct (finvS i) as [|[i' H']]; [subst; eauto|inversion i'].
+    - set (P' := (fun (i : Fin.t (S n'')) x => P (Fin.FS i) x)).
+      assert (forall i : Fin.t (S n''), exists x : T, P' i x) as Hex.
+      { intros i; subst; apply (H (Fin.FS i)). }
+      destruct (IHn' P' Hex) as [v IHP'].
+      destruct (H Fin.F1) as [x1 H1].
+      exists (x1 :: v); intros i; destruct (finvS i) as [|[i' ?]]; subst; unfold P' in *; eauto.
+  Qed.
+
+  Variable t : T.
+
+  Lemma vec_eq_ex (f : Fin.t n -> T) :
+    (forall i j : Fin.t n, f i = f j) -> (exists c, forall i : Fin.t n, f i = c).
+  Proof.
+    induction n; intros H; [exists t; intros i; inversion i | ].
+    exists (f Fin.F1); intros i; destruct (finvS i) as [| [i' ?]]; subst; eauto.
+  Qed.
+
+  Fixpoint init (n : nat) : (Fin.t n -> T) -> Vector.t T n :=
+    match n with
+      | 0 => fun _ => []
+      | S n' => fun f => (f Fin.F1) :: init (fun i => f (Fin.FS i)) 
+    end%nat.
+
+  Lemma init_spec (m : nat) (f : Fin.t m -> T) : forall i : Fin.t m, (init f)[@i] = f i.
+  Proof.
+    revert f; induction m; intros f i; [inversion i|].
+    destruct (finvS i) as [|[i' ?]]; subst; simpl; [| rewrite IHm]; eauto.
+  Qed.
+
+  Lemma vinv0 (v : Vector.t T 0) : v = [].
+  Proof.
+    pattern v; apply case0; eauto.
+  Qed.
+
+  Lemma vinvS (v : Vector.t T (S n)) : exists x y, v = x :: y.
+    pattern n, v; apply caseS.
+    intros x n1 y; repeat eexists; eauto.
+  Qed.
+End Vector.
